%!TEX program = xelate
\input{structure.tex}
\usepackage{epstopdf}
\usepackage{graphics}
\usepackage{subfig}
\usepackage{listings}
\lstset{
  numbers=left,
    framexleftmargin=10mm,
    frame=none,
    backgroundcolor=\color[RGB]{245,245,244},
  keywordstyle=\bf\color{blue},
  identifierstyle=\bf,
  numberstyle=\color[RGB]{0,192,192},
  commentstyle=\it\color[RGB]{0,96,96},
  stringstyle=\rmfamily\slshape\color[RGB]{128,0,0},
  showstringspaces=false,
  extendedchars=false
    }
\DeclareGraphicsExtensions{.eps,.ps,.jpg,.bmp}

\begin{document}
\title{Assignment 9}{}

\problem{1}{Problem 2, Page 151}
\proof{Proof}{
First, one notices that $e_0 = 0$, thus
\[
e_i = e_0 + h\sum_{j = 0}^{i-1} \delta_x^+ = h\sum_{j=0}^{i-1}\delta_x^+e_j.
\]
\qquad\qquad Using Schwarz inequality, one finds
\[
\begin{aligned}
\vt{\mathbf{e}}_{\mathnormal{l}^2}^2 &= \vt{\left(h\sum_{j=0}^{i-1}\delta_x^+e_j\right)_i}_{l^2}^2 = \sum_{i=1}^{N}\left(h\sum_{j=0}^{i-1}\delta_x^+e_j\right)^2 \leqslant \sum_{i=1}^{N}ih^2\sum_{j=0}^{i-1}\left(\delta_x^+e_j\right)^2 \n
&\leqslant N^2h^2\sum_{i=1}^{N-1}(\delta_x^+e_j)^2 = \vt{\delta_x^+\mathbf{e}}_{l^2}.
\end{aligned}
\]

\qquad\qquad So we have proved (3.1.54). Next we use this inequality to proof the convergence. \n
\qquad\qquad The truncation error of the differenced system is
\[
R_i = -\delta_x^2u(x_i) - f(x_i) = -\delta_x^2u(x_i) + \frac{d^2u}{dx^2} = 	-\frac{h^2}{12}+O(h^4).
\]
\qquad\qquad Define $e_i = u(x_i) - u_i$, then $e_i$ satisfies
\[
-\delta_x^2 e_i = R_i.
\]
\qq\qq So we have
\[
\vt{\mathbf{e}} \leqslant \vt{\sigma_x^+e} \leqslant \vt{R} \sim O(h^2).
\]
\qq\qq It means the function value is of order-2 convergent. When it comes to the derivatives,
\[
\frac{du}{dx}(x_i) = \frac{u(x_{i+1})-u(x_{i-1})}{2h} + \frac{h^2}{12}u^{(3)}(x_i) + O(h^3).
\]
\qq\qq Using the same methods we can get that the values of derivatives are of order-2 convergent.
}


\problem{2}{Problem 3, Page 151}
\proof{Proof}{
\[
-\frac{d}{dx}\left(a(x)\frac{du}{dx}\right) = -(a'(x)u'(x) + a(x)u''(x)) = f
\]
\qq\qq Thus the three-point-difference scheme is
\[
-a_i'\delta_xu_i - a_i\delta_x^2u_i = f_i.
\]
\qq\qq When $f_i \geqslant 0$, 
\[
\begin{aligned}
u_{i+1} &= 2u_i - u_{i-1} - \frac{h^2}{a_i}f_i - \frac{h_ia_i'}{a_i}\delta_xu_i \n
& \leqslant (2-\frac{h_ia_i'}{a_i})u_i - (1-\frac{h_ia_i'}{a_i})u_{i-1},
\end{aligned}
\]
\qq\qq where we used the backward scheme in the last term. According to the same process as Lemma 3.1.12, we finds that either $u_i$ being a constant, or the minimum is reached on the boarder.
}
\solution{Max-module estimation}{
We construct a problem:
\[
\left\{
\begin{aligned}
&v_0 = v_n = 0, \n
&-\delta_x(a_i\delta_xu_i) = \vt{\mathbf{R}}_{l^\infty},
\end{aligned}
\right.
\]
\qq\qq Then $v_i = \frac{1}{N}\sum_{j=1}^{i}\frac{\frac{i}{N}\vt{\mathbf{R}}_{l^\infty} + \frac{\sum_{j=1}^{N}\frac{i\vt{\mathbf{R}}_{l^\infty}}{a_i}}{\sum_{j=1}^{N}\frac{1}{a_i}}}{a_i}$.
Thus
\[
\vt{e_i} \leqslant v_i \leqslant C\vt{\mathbf{R}}_{l^\infty} \leqslant C_2h^2.
\]
}
% \refgroup{
% \reference{a a a a  a a}
% }


\end{document}