%!TEX program = xelate
\input{structure.tex}
\usepackage{epstopdf}
\usepackage{graphics}
\usepackage{subfig}
\usepackage{listings}
\lstset{
  breaklines=true,
  xleftmargin=25pt,
  xrightmargin=25pt,
  aboveskip=0pt,
  belowskip=10pt,
  basicstyle=\ttfamily,
  showstringspaces=false,
  frame=ltrb,
  tabsize=4,
  numbers=left,
  numberstyle=\small,
  numbersep=8pt,
  morekeywords={*, factorial, sum, erlang},
  keywordstyle=\color{blue!70}, commentstyle=\color{red!50!green!50!blue!50},
}
\DeclareGraphicsExtensions{.eps,.ps,.jpg,.bmp}

\begin{document}

\title{Numerical Analysis \\ Assignment 8}
\date{\today}
\author{Chuan Lu}

\maketitle

\problem{1}{Problem 3.42, Page 193}
\solution{(a)}{
Consider
$$
e^{i\frac{2\pi jk}{m}} = \cos\left(\frac{2\pi jk}{m}\right) + i\sin\left(\frac{2\pi jk}{m}\right).
$$
Then if $k$ is a multiple of $m$, we have 
$$
\sum_{j=0}^{m-1}\cos\left(\frac{2\pi jk}{m}\right) = \sum_{j=0}^{m-1}1 = m.
$$
Otherwise we have
$$
\sum_{j=0}^{m-1}\cos\left(\frac{2\pi jk}{m}\right)+i\sum_{j=0}^{m-1}\sin\left(\frac{2\pi jk}{m}\right) = \sum_{j=0}^{m}e^{i\frac{2\pi jk}{m}} = \frac{1-e^{i\frac{2\pi k}{m}m}}{1-e^{i\frac{2\pi k}{m}}} = 0.
$$
Thus
$$
\sum_{j=0}^{m-1}\cos\left(\frac{2\pi jk}{m}\right) = \sum_{j=0}^{m-1}\sin\left(\frac{2\pi jk}{m}\right) = 0.
$$
}
\solution{(b)}{
$$
\sum_{j=0}^{m-1}\cos\left(\frac{2\pi jk}{m}\right)\cos\left(\frac{2\pi jl}{m}\right) = \frac{1}{2}\sum_{j=0}^{m-1}\left(\cos\left(\frac{2\pi j(k+l)}{m}\right) + \cos\left(\frac{2\pi j(k-l)}{m}\right)\right)
= \left\{
\begin{aligned}
&m, ~k=l=\frac{m}{2} \\
&\frac{m}{2}, ~k=l\ne\frac{m}{2}, ~\text{or}~ k+l = m, k\ne l\\
&0, ~\text{others}
\end{aligned}
\right.
$$
$$
\sum_{j=0}^{m-1}\sin\left(\frac{2\pi jk}{m}\right)\sin\left(\frac{2\pi jl}{m}\right) = \frac{1}{2}\sum_{j=0}^{m-1}\left(\cos\left(\frac{2\pi j(k-l)}{m}\right) - \cos\left(\frac{2\pi j(k+l)}{m}\right)\right)
= \left\{
\begin{aligned}
&\frac{m}{2}, ~k=l\ne\frac{m}{2}\\
&-\frac{m}{2}, ~k+l=m, k\ne l \\
&0, ~\text{others}
\end{aligned}
\right.
$$
$$
\sum_{j=0}^{m-1}\cos\left(\frac{2\pi jk}{m}\right)\sin\left(\frac{2\pi jl}{m}\right) = \frac{1}{2}\sum_{j=0}^{m-1}\left(\sin\left(\frac{2\pi j(k+l)}{m}\right) + \sin\left(\frac{2\pi j(l-k)}{m}\right)\right)
= 0.
$$
}

\problem{2}{Problem 3.43, Page 194}
\solution{(a)}{
$$
d_k = \frac{1}{m}\sum_{j=0}^{m-1}w_m^{jk}x_j = \frac{1}{m}\sum_{j=0}^{m-1}e^{-i\frac{2\pi jk}{m}}.
$$
The same with Problem 1, 
$$
d_k = \left\{
\begin{aligned}
&1, ~k=0 \\
&0, ~k\ne 0
\end{aligned}
\right.
$$
}
\solution{(b)}{
$$
d_k = \frac{1}{m}\sum_{j=0}^{m-1}w_m^{jk}x_j = \frac{1}{m}\sum_{j=0}^{m-1}(-1)^ke^{-i\frac{2\pi jk}{m}} = \frac{1}{m}\frac{1-(-1)^me^{-i2\pi jk}}{1-(-1)e^{-i\frac{2\pi k}{m}}} = 
\left\{
\begin{aligned}
&1, ~k = \frac{m}{2}, ~m = 2n \\
&0, ~\text{other}~ k, ~m = 2n \\
\end{aligned}
\right.
$$
}
\solution{(c)}{
$$
d_k = \frac{1}{m}\sum_{j=0}^{m-1}je^{-i\frac{2\pi jk}{m}} = \frac{1}{e^{-i\frac{2\pi k}{m}}-1}((m-1)e^{-i2\pi k}-\frac{e^{-i\frac{2\pi k}{m}}(1-e^{-i2\pi k})}{1-e^\frac{-i2\pi k}{m}}) = 
\left\{
\begin{aligned}
&\frac{m-1}{2}, ~k=0 \\
&\frac{m-1}{e^{-i\frac{2\pi k}{m}}-1}, ~k\ne 0
\end{aligned}
\right.
$$
}

\end{document}