%!TEX program = xelate
\input{structure.tex}
\usepackage{epstopdf}
\usepackage{graphics}
\usepackage{subfig}
\usepackage{listings}
\lstset{
  breaklines=true,
  xleftmargin=25pt,
  xrightmargin=25pt,
  aboveskip=0pt,
  belowskip=10pt,
  basicstyle=\ttfamily,
  showstringspaces=false,
  frame=ltrb,
  tabsize=4,
  numbers=left,
  numberstyle=\small,
  numbersep=8pt,
  morekeywords={*, factorial, sum, erlang},
}
\DeclareGraphicsExtensions{.eps,.ps,.jpg,.bmp}

\begin{document}

\title{Numerical Analysis \\ Assignment 1}
\date{\today}
\author{Chuan}

\maketitle

\problem{1}{Problem 1.1, Page 43}
\solution{(a)}{
In fact, 
$$
\frac{1}{n} n\inf_{a\le x\le b} f(x) \le \frac{1}{n}\sum_{i=1}^{n}f(i) \le \frac{1}{n}n\sup_{a\le x\le b}f(x).
$$
So according to intermediate theorem, there exists $\zeta\in[a, b]$, $S = f(\zeta)$.
}
\solution{(b)}{
The proposition now becomes as this:
$$
S = \sum_{i=1}^{n}w_if(x_i) = f(\zeta)\sum_{i=1}^{n}w_i,
$$
for some $\zeta\in [a, b]$. The proof is just the same as (a).
}

\problem{2}{Problem 1.2, Page 43}
\solution{(a)}{
Assume $0 > x > z$, then 
$$
\begin{aligned}
\left|e^x-e^z\right| &= e^z(e^{x-z}-1) = e^z\left[(x-z) + \frac{(x-z)^2}{2} + \frac{e^{\xi}}{3!}(x-z)^3\right] \\
&= e^z(x-z)\left[1+\frac{(x-z)}{2}\right]
\end{aligned}
$$
}
\solution{(b)}{
a
}
\solution{(c)}{
Denote $\xi = x-y$, then
$$
x^p-y^p = (y+\xi)^p-y^p = py^{p-1}\xi + R, ~R > 0.
$$
and we have
$$
x^p-y^p = x^p-(x-\xi)^p = px^{p-1}\xi + R, ~R < 0.
$$
So the inequality stands.
}

\problem{3}{Problem 1.4, Page 44}
\solution{Proof}{
According to Integral Mean Value theorem, 
$$
\int_{0}^h x^2(h-x)^2g(x)dx = g(\xi)\int_{0}^h x^2(h-x)^2dx = \frac{1}{30}h^5g(\xi),
$$
for some $\xi\in [0, h]$.
}

\problem{4}{Problem 1.5, Page 44}
\solution{(a)}{
Since 
$$
\left(\int_0^x e^{-t^2}dt\right)' = e^{-x^2},
$$
and 
$$
\begin{aligned}
e^{-x^2} &= 1+(-x^2)+\frac{(-x^2)^2}{2!}+\frac{(-x^2)^3}{3!}+\cdots+\frac{(-x^2)^n}{n!}+\frac{e^{-\theta x^2}}{(n+1)!}(-x^2)^{n+1} \\ 
&= 1-x^2+\frac{x^4}{2!}-\frac{x^6}{3!}+\cdots+\frac{(-1)^nx^{2n}}{n!}+\frac{(-1)^{n+1}e^{-\theta x^2}}{(n+1)!}x^{2n+2}
\end{aligned}
$$
We have 
$$
\frac{1}{x}\int_0^x e^{-t^2}dt = \frac{1}{1\cdot0!} - \frac{1}{3\cdot 1!}x^2 + \frac{1}{5\cdot 2!}x^4 + \cdots + (-1)^{n}\frac{1}{(2n+1)\cdot n!}x^{2n} + R_{2n+1},
$$
where 
$$
|R_{2n+1}| \le \frac{x^{2n+1}}{(2n+2)(n+1)!}.
$$
}
\solution{(b)}{
Since
$$
\left(\sin^{-1}(x)\right)' = \frac{1}{\sqrt{1-x^2}},
$$
and
$$
\begin{aligned}
\frac{1}{\sqrt{1-x^2}} &= 1- \frac{1}{2}(-x^2)+\frac{1\cdot 3}{2\cdot 4}(-x^2)^2+\cdots + (-1)^n\frac{(2n-1)!!}{2n!!}(-x^2)^n + (-1)^{n+1}\frac{(2n+1)!!}{(2n+2)!!}\frac{(-x^2)^{n+1}}{(1-\theta x^2)^{n+\frac{3}{2}}} \\
&= 1 + \frac{1}{2}x^2+\frac{1\cdot 3}{2\cdot 4}x^4+\cdots + \frac{(2n-1)!!}{2n!!}x^{2n} + \frac{(2n+1)!!}{(2n+2)!!}\frac{x^{2(n+1)}}{(1-\theta x^2)^{n+\frac{3}{2}}}
\end{aligned}
$$
We have
$$
\sin^{-1}(x) = x + \frac{1}{3\cdot 2}x^3 + \frac{1\cdot 3}{5\cdot 2\cdot 4}x^5 +\cdots + \frac{(2n-1)!!}{(2n+1)(2n)!!}x^{2n+1} + R_{2n+2},
$$
where 
$$
|R_{2n+2}| \le \frac{(2n+1)!!}{(2n+2)(2n+2)!!}x^{2n+2}
$$
}
\solution{(c)}{
Since
$$

$$
}
\end{document}